cpSTLC/cpSTLCa_Props.v
@@ -135,11 +135,18 @@ Qed.
 (** **** Checking Ids' Uniqueness *)
 (* ----------------------------------------------------------------- *)
 
+(** First of all we want to prove that [ids_are_unique] is sound, 
+    i.e. if it returns true, than there is no duplicates in the list.     
+*)
+
 Theorem ids_are_unique__sound : forall (l : list id),
     IdLS.ids_are_unique l = true -> NoDup l.
 Proof.
   apply IdLS.Props.ids_are_unique__sound.
 Qed.
+
+(** And we also have to prove the opposite side, completeness.
+    If there are no dups in the list, then [ids_are_unique] gives true. *)
 
 Theorem ids_are_unique__complete : forall (l : list id),
     NoDup l -> IdLS.ids_are_unique l = true.
@@ -147,348 +154,10 @@ Proof.
   apply IdLS.Props.ids_are_unique__complete.
 Qed.
 
-(** First of all we want to prove that [ids_are_unique] is sound, 
-    i.e. if it returns true, than there is no duplicates in the list.    
 
-    A bunch of auxiliary lemmas is needed to prove the main theorem.  
-*)
 
 Section IdSetProofs.
 
-(*
-(* We need some facts from sets... *)
-
-Module IdSetFacts := MSetFacts.WFacts IdSet.
-Module IdSetProps := MSetProperties.WProperties IdSet.
-
-
-
-Import IdSet.
-Import IdSetFacts.
-Import IdSetProps.
-
-Lemma mem_empty__false : forall (x : id),
-    ids_mem x ids_empty = false.
-Proof.
-  reflexivity.
-Qed.
-
-Lemma add_eq__mem_true : forall (x : id) (s : id_set),
-    ids_mem x (ids_add x s) = true.
-Proof.
-  intros x s. rewrite mem_1.
-  reflexivity.
-  apply add_1. reflexivity.
-Qed.
-
-Lemma add_neq__mem_ignore : forall (x y : id) (s : id_set),
-    x <> y ->
-    ids_mem y (ids_add x s) = ids_mem y s.
-Proof.
-  intros x y s. intros H. 
-  remember (add_neq_iff s H) as Hneq. clear HeqHneq.
-  repeat (rewrite <- IdSet.mem_spec in Hneq). 
-  unfold ids_mem, ids_add in *.
-  destruct (IdSet.mem y s) eqn:Hmem.
-  - apply Hneq. reflexivity.
-  - destruct (IdSet.mem y (ids_add x s)) eqn:Hmem'.
-    apply Hneq in Hmem'. inversion Hmem'.
-    assumption.
-Qed.
-
-Lemma mem_add_false__mem_false : forall (x y : id) (s : id_set),
-    ids_mem y (ids_add x s) = false ->
-    ids_mem y s = false.
-Proof.
-  intros x y s H.
-  rewrite <- not_mem_iff in H.
-  rewrite <- not_mem_iff. intros Hin.
-  apply add_2 with (x := x) in Hin. auto.
-Qed.  
-
-Lemma add_elem_into_eq__eq : forall (s s' : id_set) (x : id),
-    IdSet.Equal s s' ->
-    IdSet.Equal (ids_add x s) (ids_add x s').
-Proof.
-  intros s s' x Heq.
-  unfold Equal. intros y.
-  split; intros Hin;
-    (destruct (beq_idP x y);
-       [subst; rewrite <- mem_spec;
-        apply add_eq__mem_true
-       |remember (add_3 n Hin) as Hyins;
-        apply add_2; apply Heq; assumption]).
-(* 
-add_2: forall (s : t) (x y : elt), In y s -> In y (add x s)
-add_3: forall (s : t) (x y : elt), x <> y -> In y (add x s) -> In y s 
-*)
-Qed.  
-  
-Lemma ids_are_unique_recur__eq_sets_eq : forall (l : list id) (s s' : id_set),
-    IdSet.Equal s s' ->
-    ids_are_unique_recur l s = ids_are_unique_recur l s'.
-Proof.
-  intros l.
-  induction l as [| h l' IHl'];
-    intros s s' Heq.
-  - (* l = nil *)
-    reflexivity.
-  - (* l = h :: l' *)
-    simpl.
-    destruct (ids_mem h s) eqn:Hhs.
-    + (* h in s *)
-      rewrite mem_spec in Hhs.
-      unfold Equal in Heq. apply Heq in Hhs as Hhs'.
-      rewrite <- mem_spec in Hhs'. unfold ids_mem. rewrite -> Hhs'.
-      reflexivity.
-    + (* h not in s' *)
-      rewrite <- not_mem_iff in Hhs.
-      (* unfold Equal in Heq. *)
-      destruct (ids_mem h s') eqn:Hhs'.
-      * rewrite mem_spec in Hhs'. apply Heq in Hhs'.
-        apply Hhs in Hhs'. contradiction.
-      * rewrite <- not_mem_iff in Hhs'.
-        assert (H: Equal (ids_add h s) (ids_add h s'))
-               by (apply add_elem_into_eq__eq; assumption).
-        apply IHl'. assumption.
-Qed.      
-
-Lemma ids_are_unique_recur__set_permute : forall (l : list id) (s : id_set) (x y : id),
-  ids_are_unique_recur l (ids_add x (ids_add y s))
-  = ids_are_unique_recur l (ids_add y (ids_add x s)).
-Proof.
-  intros l s x y.
-  apply ids_are_unique_recur__eq_sets_eq.
-  apply IdSetProps.add_add.
-(*
-IdSetProps.add_add: forall (s : t) (x x' : elt), Equal (add x (add x' s)) (add x' (add x s))
-*) 
-Qed.           
-
-Lemma ids_are_unique_recur_add_true__true : forall (l : list id) (s : id_set) (x : id),
-    ids_are_unique_recur l (ids_add x s) = true -> 
-    ids_are_unique_recur l s = true.
-Proof.
-  intros l. induction l as [| h l' IHl'].
-  - (* l = nil *)
-    intros. reflexivity.
-  - (* l = h :: l' *)
-    intros s x. simpl. 
-    destruct (ids_mem h (ids_add x s)) eqn:Hmem.
-    + intros Hcontra. inversion Hcontra.
-    + rewrite -> ids_are_unique_recur__set_permute.
-      apply mem_add_false__mem_false in Hmem. rewrite -> Hmem.
-      apply IHl'.
-Qed.    
-
-Lemma ids_are_unique_permute : forall (x y : id) (l : list id),
-    ids_are_unique (x :: y :: l) = ids_are_unique (y :: x :: l).
-Proof.
-  intros x y l.
-  destruct (beq_idP x y).
-  - (* x = y *)
-    subst. reflexivity.
-  - (* x <> y *)
-    unfold ids_are_unique. simpl.
-    rewrite ids_are_unique_recur__set_permute.
-    repeat (rewrite add_neq__mem_ignore; simpl).
-    reflexivity. auto. assumption.
-Qed.    
-
-Lemma ids_are_unique_recur_cons__add : forall (l : list id) 
-                                              (x : id) (s : id_set),
-    ids_mem x s = false ->
-    ids_are_unique_recur (x :: l) s 
-    = ids_are_unique_recur l (ids_add x s).
-Proof.
-  intros. simpl.
-  rewrite H. reflexivity.
-Qed.
-    
-Lemma ids_are_unique_cons : forall (x : id) (l : list id),
-    ids_are_unique (x :: l) = true ->
-    ids_are_unique l = true.
-Proof.
-  intros x [| h l'].
-  - (* l = nil *)
-    intros []. reflexivity. 
-  - (* l = h :: l' *)
-    (* intros x. *)
-    unfold ids_are_unique in *. 
-    unfold ids_mem, ids_add, ids_empty in *.
-    simpl in *.
-    destruct (beq_idP h x).
-    + (* h = x *)
-      subst h. rewrite -> add_eq__mem_true.
-      intros Hcontra. inversion Hcontra.
-    + (* h <> x *)
-      rewrite -> add_neq__mem_ignore. simpl.
-      intros H. rewrite ids_are_unique_recur__set_permute in H.
-      apply ids_are_unique_recur_add_true__true in H.
-      assumption.
-      apply not_eq_sym; assumption.
-Qed.      
-
-Lemma ids_are_unique_cons__not_in : forall (l : list id) (x : id),
-    ids_are_unique (x :: l) = true ->
-    ~ List.In x l.
-Proof.
-  intros l. induction l as [| h l'].
-  - (* l = nil *)
-    intros x _ H. inversion H. 
-  - (* l = h :: l' *)
-    intros x H Hin.
-    inversion Hin as [Hxh | Hxl'].
-    + (* h = x *)
-      subst. unfold ids_are_unique in H.
-      simpl in H. rewrite -> add_eq__mem_true in H.
-      inversion H.
-    + (* h in l' *)
-      rewrite ids_are_unique_permute in H.
-      apply ids_are_unique_cons in H.
-      apply IHl' in H. apply H in Hxl'. contradiction.
-Qed.            
-
-(* ----------------------------------------------------------------- *)
-
-(** We prove the main [ids_are_unique] soundness theorem below. *)
-
-(** And we also have to prove the opposite side, completeness.
-    If there is no dups in the list, then ids_are_unique is true. *)
-
-Lemma ids_are_unique_recur_cons : forall (l : list id) (x : id) (s : id_set),
-    ids_are_unique_recur (x :: l) s = true ->
-    ids_are_unique_recur l s = true.
-Proof.
-  intros [| h l'].
-  - (* l = nil *)
-    intros x s Hrec. reflexivity.
-  - (* l = h :: l' *)
-    intros x s Hxh.
-    inversion Hxh. rewrite -> H0.
-    destruct (ids_mem x s) eqn: Hmemxs. 
-      inversion H0.
-    destruct (ids_mem h (ids_add x s)) eqn: Hmemhxs.
-      inversion H0.
-    remember Hmemhxs as Hmemhxs'; clear HeqHmemhxs'.
-    apply ids_are_unique_recur_cons__add with (l := l') (s := (ids_add x s)) in Hmemhxs.
-    rewrite -> H0 in Hmemhxs.
-    apply ids_are_unique_recur_add_true__true in Hmemhxs.
-    assumption.
-Qed.
-
-Lemma ids_are_unique_recur_cons__mem_false : forall (l : list id) 
-                                                    (x : id) (s : id_set),
-    ids_are_unique_recur (x :: l) s = true ->
-    ids_mem x s = false.
-Proof.
-  intros [| h l'].
-  - (* l = nil *)
-    intros x s H.
-    inversion H as [H'].
-    destruct (ids_mem x s) eqn: Hxs; auto. 
-  - (* l = h :: l' *)
-    intros x s H. 
-    simpl in H. destruct (ids_mem x s) eqn: Hxs; auto.
-Qed.
-
-Lemma not_in_list_cons : forall (l : list id) (h : id) (x : id),
-    ~ List.In x (h :: l) ->
-    (~ List.In x l) /\ (x <> h).
-Proof.
-  intros l h x Hh.
-  split.
-  - (* ~ List.In x l *)
-    intros H. assert (contra: List.In x (h :: l)). 
-    { simpl. right. assumption. }
-    apply Hh in contra. auto.                                       
-  - (* x <> h *)
-    intros H. assert (contra: List.In x (h :: l)). 
-    { simpl. left. symmetry. assumption. }    
-    tauto.
-Qed.
-
-Lemma ids_are_unique_recur__not_mem_add : forall (l : list id) 
-                                                 (x : id) (s : id_set),
-    ids_are_unique_recur l s = true ->
-    ~ List.In x l ->
-    ids_mem x s = false ->
-    ids_are_unique_recur l (ids_add x s) = true.
-Proof.
-  intros l. induction l as [| h l' IHl'].
-  - (* l = nil *)
-    intros. reflexivity.
-  - (* l = h :: l' *)
-    intros x s Hrecs Hin Hmem.    
-    simpl.
-
-    assert (Hin' := Hin). apply not_in_list_cons in Hin'.
-    inversion Hin' as [Hinl' Hneqxh].
-
-    assert (Hhs: ids_mem h s = false) 
-      by (apply ids_are_unique_recur_cons__mem_false with l'; apply Hrecs).
-    assert (Hmemf: ids_mem h (ids_add x s) = false) by
-        (rewrite (add_neq__mem_ignore x h s Hneqxh); rewrite Hhs; auto).
-
-    rewrite Hmemf.
-    rewrite ids_are_unique_recur__set_permute.
-    rewrite (ids_are_unique_recur_cons__add l' h s Hhs) in Hrecs.
-
-    apply IHl'. 
-    + assumption.
-    + assumption.
-    + rewrite add_neq__mem_ignore; auto.
-Qed.
-
-Lemma ids_are_unique_recur_true__cons_true : forall (l : list id) 
-                                                    (s : id_set) (x : id),
-    ids_are_unique_recur l s = true ->
-    ~ List.In x l ->
-    ids_mem x s = false ->
-    ids_are_unique_recur (x :: l) s = true.
-Proof. 
-  intros l s x H Hin Hmem.
-  simpl.
-  rewrite Hmem.
-  apply ids_are_unique_recur__not_mem_add; auto.
-Qed.
-
-(* ----------------------------------------------------------------- *)
-
-(** Here is the main [ids_are_unique] soundness theorem: *)
-
-Theorem ids_are_unique__sound : forall (l : list id),
-    ids_are_unique l = true -> NoDup l.
-Proof.
-  intros l. induction l as [ | h l' IHl'].
-  - (* l = nil *)
-    intros H. apply NoDup_nil.
-  - (* l = h :: l' *)
-    intros H. apply ids_are_unique_cons in H as H'.
-    apply IHl' in H'.
-    apply NoDup_cons.
-    apply ids_are_unique_cons__not_in in H. assumption.
-    assumption.
-Qed.
-
-(** Here is the main [ids_are_unique] completeness theorem: *)
-
-Theorem ids_are_unique__complete : forall (l : list id),
-    NoDup l -> ids_are_unique l = true.
-Proof.
-  intros l. induction l as [ | h l' IHl'].
-  - (* l = nil *)
-    intros H. reflexivity.
-  - (* l = h :: l' *)
-    intros H. inversion H; subst.
-    apply IHl' in H3.
-    unfold ids_are_unique in *. 
-    apply ids_are_unique_recur_true__cons_true.
-    + assumption.
-    + assumption.
-    + reflexivity.
-Qed.
-*)
 
 (* ----------------------------------------------------------------- *)
 (** **** Types Validity *)
@@ -634,6 +303,25 @@ Section IdMapProofs.
 Import IdMapFacts.
 Import IdMapProps.
 
+Lemma split_fst__map_fst : forall {A B : Type} (l : list (prod A B)) 
+                                  (xs : list A) (ys : list B),
+    split l = (xs, ys) -> 
+    map fst l = xs.
+Proof.
+  intros A B l. induction l as [| h l' IHl'].
+  - (* l = nil *)
+    intros xs ys H. simpl in H. inversion H; subst.
+    reflexivity.
+  - (* l = h :: l' *)
+    intros xs ys H. destruct h eqn:eqh.
+    simpl in H. destruct (split l'). simpl. 
+    destruct xs as [| x xs']. destruct ys as [| y ys'].
+    + inversion H.
+    + inversion H.
+    + inversion H; subst. apply f_equal.
+      apply IHl' with (ys := l0). reflexivity.
+Qed.
+
 Lemma map_from_list_not_in__preserves_mapping : 
   forall (pnds : list (prod id ty)) (nm : id) (tp : ty)(m : id_map ty),  
 (* JB | cannot figure out how to write [list (id * type)], scoping problems *)
@@ -695,25 +383,6 @@ Proof.
   unfold find_ty, mids_find. 
   apply IdMap.find_1.
   apply map_from_list_add_unique__preserves_mapping. auto.
-Qed.
-
-Lemma split_fst__map_fst : forall {A B : Type} (l : list (prod A B)) 
-                                  (xs : list A) (ys : list B),
-    split l = (xs, ys) -> 
-    map fst l = xs.
-Proof.
-  intros A B l. induction l as [| h l' IHl'].
-  - (* l = nil *)
-    intros xs ys H. simpl in H. inversion H; subst.
-    reflexivity.
-  - (* l = h :: l' *)
-    intros xs ys H. destruct h eqn:eqh.
-    simpl in H. destruct (split l'). simpl. 
-    destruct xs as [| x xs']. destruct ys as [| y ys'].
-    + inversion H.
-    + inversion H.
-    + inversion H; subst. apply f_equal.
-      apply IHl' with (ys := l0). reflexivity.
 Qed.
 
 Lemma map_from_list'__eq_maps : 
